lean/Och/Simple/Std.lean
@@ -3,4 +3,7 @@ import Och.Simple.Std.Unit
 import Och.Simple.Std.Bool
 import Och.Simple.Std.Nat
 import Och.Simple.Std.Pair
+import Och.Simple.Std.DBool
+import Och.Simple.Std.DNat
+import Och.Simple.Std.Mu
 import Och.Simple.Std.Aspirational
